coq/theories/imperative/ImpProperties.v
@@ -255,45 +255,37 @@ Proof.
   induction fuel; induction c; simpl in *; intros.
   Transparent eval_cmd.
   Opaque EVAL_CMD.
+  (* Base cases: fuel = 0, EVAL_CMD 0 always returns TimeOut *)
   all: simpl in *; unfold_outcome; unfold_monadic; cleanup.
+  (* Many goals where hypothesis = goal, or trivial reflexivity *)
   all: try solve [reflexivity].
+  all: try solve [assumption].
   Opaque eval_cmd.
-  all: repeat lazymatch goal with
-  | IH: forall s res s1, eval_cmd ?c _ _ = _ -> _, H: context [ let (_, _) := eval_cmd ?c ?f ?s2 in _ ] |- _ =>
+  (* Handle compound commands - destruct intermediate results *)
+  all: repeat match goal with
+  | H: context [ let (_, _) := eval_cmd ?c ?f ?s2 in _ ] |- context [ let (_, _) := eval_cmd ?c ?f' ?s2 in _ ] =>
     let Hd := fresh "Hd" in
-    destruct (eval_cmd c f s2) eqn:Hd; subst; cleanup; specialize IH with (1 := Hd)
+    destruct (eval_cmd c f s2) eqn:Hd; subst; cleanup
   | H: context [ match ?o with _ => _ end ] |- _ => destruct o eqn:?; subst; cleanup
-  | H: eval_exp _ _ = _ |- _ =>
-    specialize eval_exp_pure with (1 := H) as ?; subst; eapply eval_exp_not_stop with (v := TimeOut) (2 := HTimeOutneqCrash) in H; eauto
-  | H: eval_exp _ _ = (_, _) |- _ =>
-    specialize eval_exp_pure with (1 := H) as ?; subst; clear H
-  | H: eval_exps _ _ = _ |- _ =>
-    specialize eval_exps_pure with (1 := H) as ?; subst; eapply eval_exps_not_stop with (v := TimeOut) (2 := HTimeOutneqCrash1) in H; eauto
-  | H: eval_test _ _ = _ |- _ =>
-    specialize eval_test_pure with (1 := H) as ?; subst; eapply eval_test_not_stop with (v := TimeOut) (2 := HTimeOutneqCrash2) in H; eauto
-  | H: EVAL_CMD 0 _ _ = _ |- _ => with_strategy transparent [EVAL_CMD] unfold EVAL_CMD in H
-  | H: Cont _ = Stop _ |- _ => inversion H; clear H; subst
-  | H: Stop TimeOut <> Stop TimeOut |- _ => congruence
+  | H: eval_test _ _ = _ |- _ => eapply eval_test_pure in H; subst
+  | H: eval_exps _ _ = _ |- _ => eapply eval_exps_pure in H; subst
   | H: (_, _) = (_, _) |- _ => inversion H; clear H; subst
-  | _ => (unfold assign, alloc, update, get_vars, get_body_and_set_vars, set_varsM,
-    catch_return, set_vars, set_memory, dest_word, get_char, put_char, set_output, inc_steps_done, add_steps_done, set_steps_done in *)
+  | H: Stop TimeOut ≠ Stop TimeOut |- _ => congruence
+  | _ => (unfold catch_return, get_vars, get_body_and_set_vars, set_varsM, assign, inc_steps_done in *)
         || unfold_outcome || unfold_monadic || (simpl in *)
   end.
-  all: unfold assign, alloc, update, get_vars, get_body_and_set_vars, set_varsM,
-    catch_return, set_vars, set_memory, dest_word, get_char, put_char, set_output, inc_steps_done, add_steps_done, set_steps_done in *.
-  all: unfold_outcome; unfold_monadic.
-  all: try solve [exists 0; rewrite Nat.add_0_r; destruct s1; simpl; eauto].
-  (* all: simpl in *; cleanup; eexists. *)
-  (* - eapply IHc2 in H; eauto; clear IHc2; rewrite IHc1; eauto; congruence.
-  - rewrite IHc1; eauto; congruence.
-  - rewrite IHc; eauto; congruence.
-  - rewrite IHc; eauto; congruence.
-  - congruence.
-  - eapply IHc2 in H; eauto; clear IHc2; rewrite IHc1; eauto; congruence.
-  - rewrite IHc1; eauto; congruence.
-  - specialize eval_test_pure with (1 := Heqp) as ?; subst.
-    rewrite IHc; try congruence; rewrite Heqp1; eauto.
-    destruct eval_cmd eqn:?; subst; cleanup.
-    rewrite IHfuel in Heqp2. ; eauto; congruence. *)
+  (* all: try solve [reflexivity].
+  (* Apply IH for base cases fuel=0 *)
+  all: try solve [eapply IHc1; eauto].
+  all: try solve [eapply IHc2; eauto].
+  all: try solve [eapply IHc; eauto].
+  (* For Seq with fuel=0: use IHc1 to rewrite first part, then IHc2 for second *)
+  1-2: specialize IHc1 with (1 := Hd) as Hc1_eq; [congruence|];
+       rewrite Hc1_eq; try (eapply IHc2; eauto).
+  (* For While with fuel=0 where body stopped *)
+  1: specialize IHc with (1 := Hd) as Hc_eq; [congruence|]; rewrite Hc_eq; reflexivity.
+  (* For Seq with fuel=S n: need IHc1 then IHc2 *)
+  1-2: specialize IHc1 with (1 := Hd) as Hc1_eq; [congruence|];
+       rewrite Hc1_eq; try (eapply IHc2; eauto). *)
+       
 Admitted.
-
